# Quadratic Equation Solution

## Problem
Solve for all values of x in simplest form:
```
13 + 3x² = 16
```

## Solution

**Step 1:** Subtract 13 from both sides
```
3x² = 16 - 13
3x² = 3
```

**Step 2:** Divide both sides by 3
```
x² = 1
```

**Step 3:** Take the square root of both sides
```
x = ±√1
x = ±1
```

## Answer
**x = 1** or **x = -1**

### Verification
- When x = 1: 13 + 3(1)² = 13 + 3 = 16 ✓
- When x = -1: 13 + 3(-1)² = 13 + 3 = 16 ✓

---

## Problem 2
Solve for all values of x in simplest form:
```
5(x² - 7) - 1 = 9
```

## Solution

**Step 1:** Expand the left side
```
5x² - 35 - 1 = 9
5x² - 36 = 9
```

**Step 2:** Add 36 to both sides
```
5x² = 9 + 36
5x² = 45
```

**Step 3:** Divide both sides by 5
```
x² = 9
```

**Step 4:** Take the square root of both sides
```
x = ±√9
x = ±3
```

## Answer
**x = 3** or **x = -3**

### Verification
- When x = 3: 5(3² - 7) - 1 = 5(9 - 7) - 1 = 5(2) - 1 = 10 - 1 = 9 ✓
- When x = -3: 5((-3)² - 7) - 1 = 5(9 - 7) - 1 = 5(2) - 1 = 10 - 1 = 9 ✓

---

## Problem 3
Solve for all values of x in simplest form:
```
15 + 3x² = 24
```

## Solution

**Step 1:** Subtract 15 from both sides
```
3x² = 24 - 15
3x² = 9
```

**Step 2:** Divide both sides by 3
```
x² = 3
```

**Step 3:** Take the square root of both sides
```
x = ±√3
```

## Answer
**x = √3** or **x = -√3**

### Verification
- When x = √3: 15 + 3(√3)² = 15 + 3(3) = 15 + 9 = 24 ✓
- When x = -√3: 15 + 3(-√3)² = 15 + 3(3) = 15 + 9 = 24 ✓
