# Quadratic Equation Solution 5

## Problem
Solve the following quadratic equation for all values of x in simplest form:

```
(x-1)² - 12 = 26
```

## Solution Steps

### Step 1: Add 12 to both sides
```
(x-1)² = 26 + 12
(x-1)² = 38
```

### Step 2: Take the square root of both sides
```
x - 1 = ±√38
```

### Step 3: Solve for x
Add 1 to both sides:
```
x = 1 ± √38
```

### Step 4: Find both solutions
```
x = 1 + √38
x = 1 - √38
```

## Final Answer

**x = 1 + √38  or  x = 1 - √38**

Note: √38 cannot be simplified further since 38 = 2 × 19 (no perfect square factors).

## Verification

### For x = 1 + √38:
```
(1 + √38 - 1)² - 12 = 26
(√38)² - 12 = 26
38 - 12 = 26
26 = 26 ✓
```

### For x = 1 - √38:
```
(1 - √38 - 1)² - 12 = 26
(-√38)² - 12 = 26
38 - 12 = 26
26 = 26 ✓
```

Both solutions are correct!

## Decimal Approximations
For reference:
- x ≈ 1 + 6.164 ≈ 7.164
- x ≈ 1 - 6.164 ≈ -5.164
