# Quadratic Equation Solution 2

## Problem
Solve the following quadratic equation for all values of x in simplest form:

```
5(x² - 4) - 5 = -5
```

## Solution Steps

### Step 1: Add 5 to both sides
```
5(x² - 4) = -5 + 5
5(x² - 4) = 0
```

### Step 2: Divide both sides by 5
```
x² - 4 = 0
```

### Step 3: Add 4 to both sides
```
x² = 4
```

### Step 4: Take the square root of both sides
```
x = ±√4
x = ±2
```

### Step 5: Find both solutions
```
x = 2
x = -2
```

## Final Answer

**x = 2  or  x = -2**

## Verification

### For x = 2:
```
5(2² - 4) - 5 = -5
5(4 - 4) - 5 = -5
5(0) - 5 = -5
0 - 5 = -5
-5 = -5 ✓
```

### For x = -2:
```
5((-2)² - 4) - 5 = -5
5(4 - 4) - 5 = -5
5(0) - 5 = -5
0 - 5 = -5
-5 = -5 ✓
```

Both solutions are correct!
