# Quadratic Equation Solution 3

## Problem
Solve the following quadratic equation for all values of x in simplest form:

```
2(x+6)² = 18
```

## Solution Steps

### Step 1: Divide both sides by 2
```
(x+6)² = 18/2
(x+6)² = 9
```

### Step 2: Take the square root of both sides
```
x + 6 = ±√9
x + 6 = ±3
```

### Step 3: Solve for x
Subtract 6 from both sides:
```
x = -6 ± 3
```

### Step 4: Find both solutions
```
x = -6 + 3 = -3
x = -6 - 3 = -9
```

## Final Answer

**x = -3  or  x = -9**

## Verification

### For x = -3:
```
2(-3 + 6)² = 18
2(3)² = 18
2(9) = 18
18 = 18 ✓
```

### For x = -9:
```
2(-9 + 6)² = 18
2(-3)² = 18
2(9) = 18
18 = 18 ✓
```

Both solutions are correct!
